\documentclass[english]{tktltiki}
\usepackage[pdftex]{graphicx}
\usepackage{subfigure}
\usepackage{booktabs}
\usepackage{url}
\usepackage{amsthm,amssymb}
 \usepackage{amsmath}
 \usepackage{enumerate}
 
 \usepackage{chngcntr}
\counterwithin*{equation}{section}
\counterwithin*{equation}{subsection}

\begin{document}
\onehalfspacing

\title{Workshop 6}
\author{Péter Ivanics}
\date{\today}

\maketitle

\section{Problem 1}
\begin{enumerate}[a)]
	\item $p_0 \rightarrow p_1 = \neg p_0 \vee p_1$
	
	Clauses: $\{\neg p_0, p_1\}$	
	
	\item $p_0 \vee (p_1 \wedge p_2)$ \\ 
	
		\begin{center}
		\begin{tabular}{c|c|c||c}
		\toprule
		$p_0$ & $p_1$ & $p_2$ &  $p_0 \vee (p_1 \wedge p_2)$ \\ 
		\midrule
		0 & 0 &  0 & 0  \\
		0 & 0 &  1 & 0 \\
		0 & 1 &  0 & 0 \\
		0 & 1 &  1 & 1 \\
		1 & 0 &  0 & 1 \\
		1 & 0 &  1 & 1 \\
		1 & 1 &  0 & 1 \\		
		1 & 1 &  1 & 1
		\end{tabular}
		\end{center}
		
		In CNF: 
		\begin{eqnarray*}
			\neg (\neg p_0 \neg p_1 \neg p_2) \wedge \neg (\neg p_0 \neg p_1 p_2) \wedge \neg(\neg p_0 p_1 \neg p_2) = \\ 
			(p_0 \vee p_1 \vee p_2) \wedge (p_0 \vee p_1 \vee \neg p_2) \wedge (p_0 \vee \neg p_1 \vee p_2)
		\end{eqnarray*}
		
		Clauses: $\{p_0, p_1, p_2\}, \{p_0, p_1, \neg p_2\}, \{p_0, \neg p_1, p_2\}$
		
	\item $\neg (p_0 \vee p_1 \vee p_2) = \neg p_0 \wedge \neg p_1 \wedge \neg p_2$
	
	Clauses: $\{\neg p_0\}, \{\neg p_1\}, \{\neg p_2\}$
	\item $(p_0 \rightarrow p_1) \rightarrow (p_1 \rightarrow p_2)$
	
			\begin{center}
		\begin{tabular}{c|c|c||c|c||c}
		\toprule
		$p_0$ & $p_1$ & $p_2$ & $(p_0 \rightarrow p_1)$ & $(p_1 \rightarrow p_2)$ & $(p_0 \rightarrow p_1) \rightarrow (p_1 \rightarrow p_2)$\\ 
		\midrule
		0 & 0 & 0 & 1 & 1 & 1 \\
		0 & 0 & 1 & 1 & 1 & 1 \\
		0 & 1 & 0 & 1 & 0 & 0 \\
		0 & 1 & 1 & 1 & 1 & 1 \\
		1 & 0 & 0 & 0 & 1 & 1 \\
		1 & 0 & 1 & 0 & 1 & 1 \\
		1 & 1 & 0 & 1 & 0 & 0 \\		
		1 & 1 & 1 & 1 & 1 & 1
		\end{tabular}
		\end{center}
		
		In CNF: 
		\begin{eqnarray*}
			\neg (\neg p_0 p_1 \neg p_2) \wedge \neg (p_0 p_1 \neg p_2) = \\
			(p_0 \vee \neg p_1 \vee p_2) \wedge (\neg p_0 \vee \neg p_1 \vee p_2)
		\end{eqnarray*}
		
		Clauses: $\{p_0, \neg p_1, p_2\}, \{\neg p_0, \neg p_1, p_2\}$
\end{enumerate}

\section{Problem 2}
\begin{enumerate}[a)]
	\item $\{p_0, p_1, \neg p_2\}$ and $\{p_2, p_3\}$:
	\begin{enumerate}[1.]
		\item $\{p_0, p_1, \neg p_2\}$ (assumption)
		\item $\{p_2, p_3\}$ (assumption)
		\item $\{p_0, p_1, p_3\}$
	\end{enumerate}
	\item $\{p_0, \neg p_0\}$ and $\{p_0, \neg p_0\}$:
		\begin{enumerate}[1.]
			\item $\{p_0, \neg p_0\}$ (assumption)
			\item $\{p_0, \neg p_0\}$ (assumption)
			\item $\varnothing$
		\end{enumerate}
	\item $\{p_0, \neg p_1, p_2\}$ and $\{\neg p_0, p_1\}$:
		\begin{enumerate}[1.]
			\item $\{p_0, \neg p_1, p_2\}$ (assumption)
			\item $\{\neg p_0, p_1\}$ (assumption)
			\item $\{\neg p_1, p_2\}$ (eliminated $p_0$)
			\item $\{p_2\}$ (eliminated $p_1$)
		\end{enumerate}
	\item $\{p_0, p_1, p_2\}$ and $\{p_2, \neg p_3, \neg p_4\}$:
		\begin{enumerate}[1.]
			\item $\{p_0, p_1, p_2\}$ (assumption)
			\item $\{p_2, \neg p_3, \neg p_4\}$ (assumption)
			\item $\{p_0, p_1, p_2, \neg p_3, \neg p_4\}$
		\end{enumerate}
\end{enumerate}

\section{Problem 3}
First, we derive the clauses from the formulas, as follows: 
\begin{eqnarray}
	p_0 & \implies & \{p_0\} \\
	p_0 \rightarrow p_1 = \neg p_0 \vee p_1 &\implies & \{\neg p_0, p_1\} \\
	(p_0 \rightarrow p_1) \rightarrow (p_1 \rightarrow p_2) &\implies & \{p_0, \neg p_1, p_2\}, \{\neg p_0, \neg p_1, p_2\}
\end{eqnarray}

Then, we use the resolution rule to conclude the solution:
\begin{itemize}
	\item $\{\neg p_1, p_2\}$	 (from 3)
	\item $\{p_1\}$ (from 1 and 2)
	\item $\{p_2\}$	(from the intermediate conclusions above)
\end{itemize}

\section{Problem 4}
First, we transform the assumptions to conjunctive normal form and then to clauses, as follows: 

\begin{eqnarray}
	\neg p_0 \rightarrow p_1 = p_0 \vee p_1 &\implies & \{p_0, p_1\} \\
	p_1 \rightarrow p_0 = \neg p_1 \vee p_0  & \implies & \{\neg p_1, p_0 \}\\
	p_0 \rightarrow (p_2 \wedge p_3) = \neg p_0 \vee (p_2 \wedge p_3) & \implies & \{ \neg p_0 \}, \{p_2, p_3\} \\
	\neg p_0 & \implies & \{\neg p_0 \}\\
	\neg p_2 & \implies & \{\neg p_2 \}\\
	\neg p_3 & \implies & \{\neg p_3\}
\end{eqnarray}

Note that the clause $\{ \neg p_0 \}$ is duplicated and therefore these clauses can be combined. Then, we use the resolution rule on items: 

\begin{itemize}
	\item $\{p_0\}$ (from 1 and 2)
	\item $\varnothing$ (from the item above and 4)
	\item $\{ p_3 \}$ (from 3 and 5)
	\item $\varnothing$ (from the item above and 6)
\end{itemize}

\lastpage

\end{document}